Make changes to get nulls working fine

ind/Gpointers.fst
@@ -1,19 +1,1 @@
 module Gpointers
-
-open LowStar.Buffer
-module HS = FStar.HyperStack
-module ST = FStar.HyperStack.ST
-module B = LowStar.Buffer
-module BO = LowStar.BufferOps
-module Mod = LowStar.Modifies
-
-let null #t : pointer_or_null t = B.null #t
-
-assume val is_null (p:pointer_or_null 't) : Tot (b:bool{b <==> p == null})
-let is_not_null (p:pointer_or_null 't) = not (is_null p)
-
-let lemma_is_null (p:pointer_or_null 't) :
-  Lemma
-    (ensures (is_null p <==> B.g_is_null p))
-    [SMTPat (is_null p)]
-    = B.null_unique p
